working desc lemma

Veritas.SparseMerkleVerifier.fst
@@ -373,7 +373,6 @@ let rec lemma_cache_contains_implies_last_add_before_evict (l:verifiable_log) (a
         (ensures (has_some_add l a /\
                   (has_some_evict l a ==> last_evict_idx l a < last_add_idx l a)))
         (decreases (length l)) 
-        [SMTPat (cache_contains (cache_at_end l) a)]
         = 
   let n = length l in
   let cache = cache_at_end l in
@@ -573,114 +572,39 @@ let desc_child (d:merkle_addr) (a:merkle_addr{is_proper_desc d a}) :
   lemma_proper_desc_left_or_right d a;
   if is_desc d (LeftChild a) then LeftChild a else RightChild a
 
-type pair = 
-  | MkPair: fst:eac_log -> snd:merkle_non_root_addr -> pair
+let changes_lemma_desc_hash_implies_add_conditions 
+  (e: verifier_log_entry)
+  (a: merkle_addr)
+  (d: merkle_addr) = 
+  match e with 
+  | MemoryOp _ -> false
+  | Evict _ _ -> false
+  | Add a1 v1 a1_anc -> a1 = a || 
+                        a1_anc = a ||
+                        a1 = d
 
-let find_recursion_add_lemma_desc_hash 
-    (l: eac_log{length l > 0 /\ is_add l (length l - 1)}) 
-    (c: merkle_non_root_addr {cache_contains_l l (parent c) /\
-                              Desc? (desc_hash_l l c) /\ 
-                              (not (is_desc (Desc?.a (desc_hash_l l c)) c) \/ 
-                               not (has_some_add l (Desc?.a (desc_hash_l l c))))})
- : ( lc:pair {length (MkPair?.fst lc) < length l /\ 
-              cache_contains_l (MkPair?.fst lc) (parent (MkPair?.snd lc)) /\
-                              Desc? (desc_hash_l (MkPair?.fst lc) (MkPair?.snd lc)) /\ 
-                              (not (is_desc (Desc?.a (desc_hash_l (MkPair?.fst lc) (MkPair?.snd lc))) (MkPair?.snd lc)) \/ 
-                               not (has_some_add (MkPair?.fst lc) (Desc?.a (desc_hash_l (MkPair?.fst lc) (MkPair?.snd lc)))))
- }) = 
- let n = length l in
- let a = parent c in 
- let cache = cache_at_end l in
- let d = Desc?.a (desc_hash_l l c) in 
- let e = index l (n - 1) in
- let l' = prefix l (n - 1) in
- let cache' = cache_at_end l' in
- match e with
- | Add a1 v1 a1_anc ->        
-      if a1 = a then (        
-        
-        (* desc_hash of a1_anc the validates a *)
-        let dh_anc = get_desc_hash a a1_anc (cached_payload_l l' a1_anc) in
-        if Empty? dh_anc then (
-          assert (is_empty_or_null a1 v1);
-          assert (v1 = Some?.v (cache a));
-          assert (v1 = cached_payload_l l a);
-          assert (Desc? (desc_hash_c c v1));
-          match c with
-          | LeftChild p -> assert (Desc? (desc_hash_c c v1)); admit()
-          | RightChild p -> admit()
-          // | _ -> 
-          (*
-          match c with 
-          | LeftChild p -> //assert (Desc? (desc_hash_c c v1)); 
-                           admit()
-          | RightChild p -> 
-          *)
-          //admit()
-        )
-        else
-          admit()
-        (*
-        if Desc?.a dh_anc <> a then (
-          
-          (* this implies that v is empty and a1_anc points to d *)
-          let c' = desc_child a a1_anc in
-
-          (* if d is not a descendant of a1_anc, we can recurse with a1_anc and l' *)
-          if not (is_desc d c') then
-            MkPair l' c'
-          else (
-            (* else, we know that d does not have an add in l, so not in l' either *)
-            lemma_not_exists_prefix (is_add_of_addr d) l (n - 1);
-            (* with recursion we get the hash collision *)
-            MkPair l' c'
-          )
-          admit()
-        )
-
-        else admit()   if not (has_some_add l' a) then 
-          MkPair l' (desc_child a a1_anc)
-                
-        else (
-          (* if a had a previous add, then it implies it had a previous evict *)
-          lemma_not_contains_implies_last_evict_before_add l' a;
-          assert (has_some_evict l' a);
-
-          (* the last evict index of a *)
-          let ie = last_evict_idx l' a in
-          let l_e = prefix l ie in
-          let cache_e = cache_at_end l_e in
-          lemma_evict_requires_cache l ie;
-
-          (* from evict add consistency a pointed to d at the time of evict *)          
-          if not (is_desc d c) then
-            MkPair l_e c
-          else (
-            (* else, we know that d does not have an add in l, so not in l_e either *)
-            lemma_not_exists_prefix (is_add_of_addr d) l ie;
-            (* with recursion we get the hash collision *)
-            MkPair l_e c
-          )
-        )
-
-        *)
-      )
-      else if not (is_desc d c) then
-        MkPair l' c
-      else if a1 = d then (
-        lemma_last_index_last_elem_sat (is_add_of_addr d) l;
-        MkPair l' c
-      )
-      else if a1_anc = a then (
-        assert (not (is_desc a1 c));
-        lemma_not_exists_prefix (is_add_of_addr d) l (n - 1);
-        MkPair l' c        
-      )
-      else (
-        assert (desc_hash_l l' c = desc_hash_l l c);
-        lemma_not_exists_prefix (is_add_of_addr d) l (n - 1);
-        MkPair l' c 
-      )     
+let lemma_prefix_recurse_lemma_desc_hash_implies_add
+    (l: eac_log) 
+    (c: merkle_non_root_addr)
+ : Lemma (requires (length l > 0 /\ 
+                    cache_contains_l l (parent c) /\
+                    Desc? (desc_hash_l l c) /\ 
+                    (not (is_desc (Desc?.a (desc_hash_l l c)) c) \/ 
+                     not (has_some_add l (Desc?.a (desc_hash_l l c)))) /\
+                    not (changes_lemma_desc_hash_implies_add_conditions (index l (length l - 1))
+                                                                         (parent c)
+                                                                         (Desc?.a (desc_hash_l l c)))))
+         (ensures (cache_contains_l (prefix l (length l - 1)) (parent c) /\
+                   Desc? (desc_hash_l (prefix l (length l - 1)) c) /\ 
+                   (not (is_desc (Desc?.a (desc_hash_l (prefix l (length l - 1)) c)) c) \/ 
+                    not (has_some_add l (Desc?.a (desc_hash_l (prefix l (length l - 1)) c)))))) =                     
+  let n = length l in
+  let d = Desc?.a (desc_hash_l l c) in
+  let l' = prefix l (n - 1) in
+  if not (is_desc d c) then ()
+  else 
+    lemma_not_exists_prefix (is_add_of_addr d) l (n - 1)
+  
 
 let rec lemma_desc_hash_implies_add 
     (l: eac_log) 
@@ -694,10 +618,16 @@ let rec lemma_desc_hash_implies_add
   let cache = cache_at_end l in
   let d = Desc?.a (desc_hash_l l c) in
   if n = 0 then SCollision (SMkLeaf Null) (SMkLeaf Null)
-  else
+  else (
     let e = index l (n - 1) in
     let l' = prefix l (n - 1) in
     let cache' = cache_at_end l' in
+
+    if not (changes_lemma_desc_hash_implies_add_conditions e a d) then (    
+      lemma_prefix_recurse_lemma_desc_hash_implies_add l c;
+      lemma_desc_hash_implies_add l' c
+    )
+    else (
     match e with
     | Add a1 v1 a1_anc ->       
       if a1 = a then (        
@@ -760,22 +690,9 @@ let rec lemma_desc_hash_implies_add
         lemma_not_exists_prefix (is_add_of_addr d) l (n - 1);
         lemma_desc_hash_implies_add l' c 
       )  
-    | MemoryOp _ ->
-      if not (is_desc d c) then 
-        lemma_desc_hash_implies_add l' c                                        
-      else (
-        lemma_not_exists_prefix (is_add_of_addr d) l (n - 1);
-        lemma_desc_hash_implies_add l' c
-      )
-    | Evict _ _ -> admit()
-      (*
-      if not (is_desc d c) then 
-        lemma_desc_hash_implies_add l' c                                        
-      else (
-        lemma_not_exists_prefix (is_add_of_addr d) l (n - 1);
-        lemma_desc_hash_implies_add l' c
-      )*)
-    
+  )
+)
+
 let rec lemma_desc_hash_empty_implies_no_desc 
   (l: verifiable_log) 
   (c: merkle_non_root_addr {cache_contains_l l (parent c) /\ has_some_add l (parent c)}) 
